Tactics.v
@@ -201,5 +201,5 @@ Ltac erewrite_anywhere f :=
 
 Ltac destruct_eq H :=
   match H with
-  | ?a = ?b => let fresh_H := fresh "Heq" in pose proof (PeanoNat.Nat.eq_dec a b) as [Heq | Heq]
+  | ?a = ?b => let fresh_H := fresh "Heq" in pose proof (PeanoNat.Nat.eq_dec a b) as [fresh_H | fresh_H]
   end.
